<?xml version="1.0" encoding="UTF-8"?>
<rdf:RDF
   xmlns:dcterms="http://purl.org/dc/terms/"
   xmlns:doap="http://usefulinc.com/ns/doap#"
   xmlns:owl="http://www.w3.org/2002/07/owl#"
   xmlns:prov="http://www.w3.org/ns/prov#"
   xmlns:rdf="http://www.w3.org/1999/02/22-rdf-syntax-ns#"
   xmlns:rdfs="http://www.w3.org/2000/01/rdf-schema#"
   xmlns:sdo="http://schema.org/"
   xmlns:skos="http://www.w3.org/2004/02/skos/core#"
>
  <rdf:Description rdf:nodeID="f7656e68342664385b4e3faded1cecac5b11">
    <rdf:first rdf:resource="http://www.w3.org/ns/ssn/ext/ObservationCollection"/>
    <rdf:rest rdf:resource="http://www.w3.org/1999/02/22-rdf-syntax-ns#nil"/>
  </rdf:Description>
  <rdf:Description rdf:nodeID="ub1bL254C19">
    <rdf:type rdf:resource="http://www.w3.org/2002/07/owl#Restriction"/>
    <owl:cardinality rdf:datatype="http://www.w3.org/2001/XMLSchema#nonNegativeInteger">1</owl:cardinality>
    <owl:onProperty rdf:resource="http://linked.data.gov.au/def/plot/stratum"/>
  </rdf:Description>
  <rdf:Description rdf:about="http://linked.data.gov.au/def/plot/stratum">
    <rdfs:label>stratum classification</rdfs:label>
    <rdfs:range rdf:resource="http://www.w3.org/2004/02/skos/core#Concept"/>
    <rdfs:subPropertyOf rdf:resource="http://purl.org/dc/terms/type"/>
    <rdf:type rdf:resource="http://www.w3.org/2002/07/owl#ObjectProperty"/>
  </rdf:Description>
  <rdf:Description rdf:about="http://www.w3.org/ns/locn#geometry">
    <rdfs:subPropertyOf rdf:resource="http://www.w3.org/ns/sosa/hasResult"/>
  </rdf:Description>
  <rdf:Description rdf:about="http://linked.data.gov.au/def/plot/SiteStratumTaxon">
    <rdfs:comment>Community of a single taxon in an identified stratum in a vegetation ecosystem occurring at an observation site</rdfs:comment>
    <rdfs:subClassOf rdf:resource="http://www.w3.org/ns/sosa/Sample"/>
    <rdfs:subClassOf rdf:nodeID="ub1bL248C19"/>
    <rdf:type rdf:resource="http://www.w3.org/2002/07/owl#Class"/>
    <rdfs:label>Single taxon community</rdfs:label>
    <rdfs:subClassOf rdf:nodeID="ub1bL254C19"/>
    <rdfs:subClassOf rdf:nodeID="ub1bL229C19"/>
    <rdfs:subClassOf rdf:nodeID="ub1bL259C19"/>
    <rdfs:subClassOf rdf:nodeID="ub1bL235C19"/>
    <rdfs:subClassOf rdf:nodeID="ub1bL242C19"/>
  </rdf:Description>
  <rdf:Description rdf:about="http://usefulinc.com/ns/doap#repository">
    <rdfs:subPropertyOf rdf:resource="http://www.w3.org/ns/prov#used"/>
  </rdf:Description>
  <rdf:Description rdf:about="http://linked.data.gov.au/def/plot/taxon">
    <rdfs:range rdf:resource="http://www.w3.org/2004/02/skos/core#Concept"/>
    <rdf:type rdf:resource="http://www.w3.org/2002/07/owl#ObjectProperty"/>
    <rdfs:subPropertyOf rdf:resource="http://purl.org/dc/terms/type"/>
    <rdfs:label>taxon classification</rdfs:label>
  </rdf:Description>
  <rdf:Description rdf:nodeID="ub1bL62C19">
    <rdf:type rdf:resource="http://www.w3.org/2002/07/owl#Restriction"/>
    <owl:onProperty rdf:resource="http://linked.data.gov.au/def/plot/mapScale"/>
    <owl:maxCardinality rdf:datatype="http://www.w3.org/2001/XMLSchema#nonNegativeInteger">1</owl:maxCardinality>
  </rdf:Description>
  <rdf:Description rdf:about="http://linked.data.gov.au/def/plot/x/Survey">
    <rdfs:subClassOf rdf:nodeID="ub1bL442C19"/>
    <rdfs:subClassOf rdf:nodeID="ub1bL452C19"/>
    <skos:editorialNote>Do we need an association between Survey and SiteVisit?</skos:editorialNote>
    <rdfs:label>Survey</rdfs:label>
    <skos:editorialNote>Do we also need Survey to be classified by: - data theme?</skos:editorialNote>
    <rdfs:subClassOf rdf:nodeID="ub1bL447C19"/>
    <rdfs:subClassOf rdf:nodeID="ub1bL464C19"/>
    <rdfs:subClassOf rdf:nodeID="ub1bL458C19"/>
    <rdfs:subClassOf rdf:resource="http://www.w3.org/ns/prov#Activity"/>
    <rdfs:subClassOf rdf:nodeID="ub1bL436C19"/>
    <rdfs:subClassOf rdf:nodeID="ub1bL430C19"/>
    <rdfs:comment>Survey is composed of a set of Observations and ObservationCollections, which may have a site as its feature-of-interest&#13;
In this context the value of feature-of-interest is expected to be the value of the chain   (ssn-ext:hasMember)+/sosa:hasFeatureOfInterest</rdfs:comment>
    <rdf:type rdf:resource="http://www.w3.org/2002/07/owl#Class"/>
  </rdf:Description>
  <rdf:Description rdf:about="http://linked.data.gov.au/def/plot/Location">
    <rdfs:subClassOf rdf:resource="http://purl.org/dc/terms/Location"/>
    <rdfs:subClassOf rdf:nodeID="ub1bL87C19"/>
    <rdfs:label>Location</rdfs:label>
    <rdfs:subClassOf rdf:nodeID="ub1bL62C19"/>
    <rdfs:comment>Location together with information about how it was obtained</rdfs:comment>
    <rdfs:subClassOf rdf:nodeID="ub1bL72C19"/>
    <rdf:type rdf:resource="http://www.w3.org/2002/07/owl#Class"/>
    <rdfs:subClassOf rdf:nodeID="ub1bL77C19"/>
    <rdfs:subClassOf rdf:nodeID="ub1bL82C19"/>
    <rdfs:subClassOf rdf:nodeID="ub1bL67C19"/>
  </rdf:Description>
  <rdf:Description rdf:nodeID="ub1bL27C19">
    <sdo:memberOf rdf:nodeID="ub1bL31C20"/>
    <sdo:identifier rdf:resource="https://orcid.org/0000-0002-3884-3420"/>
    <rdf:type rdf:resource="http://schema.org/Person"/>
    <sdo:email>simon.cox@csiro.au</sdo:email>
    <sdo:name>Simon J.D.Cox</sdo:name>
  </rdf:Description>
  <rdf:Description rdf:nodeID="f7656e68342664385b4e3faded1cecac5b8">
    <rdf:first rdf:resource="http://www.opengis.net/ont/geosparql#Geometry"/>
    <rdf:rest rdf:nodeID="f7656e68342664385b4e3faded1cecac5b9"/>
  </rdf:Description>
  <rdf:Description rdf:nodeID="ub1bL304C19">
    <owl:onProperty rdf:resource="http://linked.data.gov.au/def/plot/hadSubActivity"/>
    <owl:someValuesFrom rdf:nodeID="ub1bL307C26"/>
    <rdf:type rdf:resource="http://www.w3.org/2002/07/owl#Restriction"/>
  </rdf:Description>
  <rdf:Description rdf:nodeID="ub1bL235C19">
    <owl:onProperty rdf:resource="http://www.w3.org/ns/sosa/isSampleOf"/>
    <rdfs:comment>relation to the Site for which this SiteStratumTaxon represents the community of a single taxon within a single stratum</rdfs:comment>
    <owl:onClass rdf:resource="http://linked.data.gov.au/def/plot/Site"/>
    <owl:minQualifiedCardinality rdf:datatype="http://www.w3.org/2001/XMLSchema#nonNegativeInteger">1</owl:minQualifiedCardinality>
    <rdf:type rdf:resource="http://www.w3.org/2002/07/owl#Restriction"/>
  </rdf:Description>
  <rdf:Description rdf:nodeID="ub1bL259C19">
    <rdf:type rdf:resource="http://www.w3.org/2002/07/owl#Restriction"/>
    <owl:onProperty rdf:resource="http://www.w3.org/ns/sosa/isFeatureOfInterestOf"/>
    <owl:minCardinality rdf:datatype="http://www.w3.org/2001/XMLSchema#nonNegativeInteger">1</owl:minCardinality>
  </rdf:Description>
  <rdf:Description rdf:nodeID="ub1bL436C19">
    <owl:someValuesFrom rdf:resource="http://www.w3.org/ns/prov#Organization"/>
    <owl:onProperty rdf:resource="http://www.w3.org/ns/prov#wasAssociatedWith"/>
    <rdfs:comment>link to organization instead of plot:Dataset class?</rdfs:comment>
    <rdf:type rdf:resource="http://www.w3.org/2002/07/owl#Restriction"/>
  </rdf:Description>
  <rdf:Description rdf:about="http://linked.data.gov.au/def/plot/x/sampleType">
    <rdfs:domain rdf:resource="http://linked.data.gov.au/def/plot/Site"/>
    <rdfs:label>sample type classification</rdfs:label>
    <rdf:type rdf:resource="http://www.w3.org/2002/07/owl#ObjectProperty"/>
    <rdfs:range rdf:resource="http://www.w3.org/2004/02/skos/core#Concept"/>
    <rdfs:subPropertyOf rdf:resource="http://purl.org/dc/terms/type"/>
    <rdfs:comment>The site's plot shape description, e.g. square, circle, etc.</rdfs:comment>
  </rdf:Description>
  <rdf:Description rdf:about="http://linked.data.gov.au/def/plot/">
    <dcterms:modified rdf:datatype="http://www.w3.org/2001/XMLSchema#date">2019-06-19</dcterms:modified>
    <owl:imports rdf:resource="http://purl.org/dc/elements/1.1/"/>
    <rdfs:label>The PLOT ontology</rdfs:label>
    <dcterms:license rdf:resource="http://creativecommons.org/publicdomain/zero/1.0/"/>
    <rdf:type rdf:resource="http://www.w3.org/2002/07/owl#Ontology"/>
    <dcterms:created rdf:datatype="http://www.w3.org/2001/XMLSchema#date">2019-03-25</dcterms:created>
    <rdfs:seeAlso rdf:resource="https://www.publish.csiro.au/book/5230/"/>
    <prov:wasGeneratedBy rdf:nodeID="ub1bL51C23"/>
    <dcterms:description>This vocabulary provides a set of classes to support capture of plot- and site-based ecological survey data. It is primary related to vegetation surveys, following the methdologies outlined in the Australian Soil and Land Survey Field Handbook. &#13;
&#13;
PLOT is technically an extension to the W3C SSN/SOSA vocabulary, and also uses elements from the SSN-EXT ontology.</dcterms:description>
    <dcterms:creator rdf:nodeID="ub1bL27C19"/>
    <rdfs:seeAlso rdf:resource="https://www.w3.org/TR/vocab-ssn-ext/"/>
    <owl:imports rdf:resource="http://www.w3.org/ns/ssn/ext"/>
    <rdfs:seeAlso rdf:resource="https://www.w3.org/ns/ssn/"/>
  </rdf:Description>
  <rdf:Description rdf:nodeID="ub1bL276C19">
    <owl:onProperty rdf:resource="http://linked.data.gov.au/def/plot/taxon"/>
    <rdf:type rdf:resource="http://www.w3.org/2002/07/owl#Restriction"/>
    <owl:cardinality rdf:datatype="http://www.w3.org/2001/XMLSchema#nonNegativeInteger">1</owl:cardinality>
  </rdf:Description>
  <rdf:Description rdf:nodeID="f7656e68342664385b4e3faded1cecac5b4">
    <rdf:rest rdf:nodeID="f7656e68342664385b4e3faded1cecac5b5"/>
    <rdf:first rdf:resource="http://www.w3.org/ns/sosa/Observation"/>
  </rdf:Description>
  <rdf:Description rdf:about="http://linked.data.gov.au/def/plot/OrganismOccurence">
    <rdfs:subClassOf rdf:nodeID="ub1bL119C19"/>
    <rdfs:subClassOf rdf:nodeID="ub1bL114C19"/>
    <rdfs:subClassOf rdf:resource="http://www.opengis.net/ont/geosparql#SpatialObject"/>
    <rdfs:comment>Organism occurrence at some specified time and place. &#13;
&#13;
1. sub-class of Sample because observations of an organism occurrence are primarily interesting if they represents a commuity or assemblage&#13;
2. sub-class of SpatialObject because it is bound to a specified location&#13;
3. sub-class of TemporalEntity because it is bound to a specified time</rdfs:comment>
    <owl:equivalentClass rdf:resource="http://rs.tdwg.org/dwc/terms/Occurrence"/>
    <rdfs:subClassOf rdf:nodeID="ub1bL108C19"/>
    <rdfs:subClassOf rdf:resource="http://www.w3.org/2006/time#TemporalEntity"/>
    <rdfs:label>Organism Occurrence </rdfs:label>
    <rdf:type rdf:resource="http://www.w3.org/2002/07/owl#Class"/>
    <rdfs:subClassOf rdf:nodeID="ub1bL124C19"/>
    <rdfs:subClassOf rdf:resource="http://www.w3.org/ns/sosa/Sample"/>
  </rdf:Description>
  <rdf:Description rdf:nodeID="ub1bL213C19">
    <owl:onProperty rdf:resource="http://linked.data.gov.au/def/plot/stratum"/>
    <owl:cardinality rdf:datatype="http://www.w3.org/2001/XMLSchema#nonNegativeInteger">1</owl:cardinality>
    <rdf:type rdf:resource="http://www.w3.org/2002/07/owl#Restriction"/>
  </rdf:Description>
  <rdf:Description rdf:nodeID="ub1bL307C26">
    <owl:unionOf rdf:nodeID="f7656e68342664385b4e3faded1cecac5b3"/>
    <rdf:type rdf:resource="http://www.w3.org/2002/07/owl#Class"/>
  </rdf:Description>
  <rdf:Description rdf:nodeID="ub1bL114C19">
    <owl:onProperty rdf:resource="http://www.opengis.net/ont/geosparql#defaultGeometry"/>
    <rdf:type rdf:resource="http://www.w3.org/2002/07/owl#Restriction"/>
    <owl:allValuesFrom rdf:resource="http://www.w3.org/2003/01/geo/wgs84_pos#Point"/>
  </rdf:Description>
  <rdf:Description rdf:about="http://linked.data.gov.au/def/plot/hadSubActivity">
    <rdfs:label>pointer to child activity</rdfs:label>
    <rdfs:domain rdf:resource="http://www.w3.org/ns/prov#Activity"/>
    <rdfs:range rdf:resource="http://www.w3.org/ns/prov#Activity"/>
    <rdf:type rdf:resource="http://www.w3.org/2002/07/owl#ObjectProperty"/>
    <rdfs:comment>To allow links between observations or site-visits and projects, programs and initiatives, between observations and site-visits, etc</rdfs:comment>
  </rdf:Description>
  <rdf:Description rdf:about="http://linked.data.gov.au/def/plot/x/sampler">
    <rdfs:subPropertyOf rdf:resource="http://www.w3.org/ns/sosa/madeBySampler"/>
    <rdf:type rdf:resource="http://www.w3.org/2002/07/owl#ObjectProperty"/>
    <rdfs:label>Sampler</rdfs:label>
    <rdfs:subPropertyOf rdf:resource="http://www.w3.org/ns/prov#wasAssociatedWith"/>
  </rdf:Description>
  <rdf:Description rdf:nodeID="ub1bL281C19">
    <owl:minCardinality rdf:datatype="http://www.w3.org/2001/XMLSchema#nonNegativeInteger">1</owl:minCardinality>
    <owl:onProperty rdf:resource="http://www.w3.org/ns/sosa/isFeatureOfInterestOf"/>
    <rdf:type rdf:resource="http://www.w3.org/2002/07/owl#Restriction"/>
  </rdf:Description>
  <rdf:Description rdf:about="http://linked.data.gov.au/def/plot/Site">
    <rdf:type rdf:resource="http://www.w3.org/2000/01/rdf-schema#Class"/>
    <rdfs:subClassOf rdf:nodeID="ub1bL145C19"/>
    <rdfs:subClassOf rdf:nodeID="ub1bL192C19"/>
    <rdfs:subClassOf rdf:nodeID="ub1bL157C19"/>
    <rdfs:subClassOf rdf:nodeID="ub1bL182C19"/>
    <rdfs:subClassOf rdf:nodeID="ub1bL165C19"/>
    <rdfs:subClassOf rdf:nodeID="ub1bL197C19"/>
    <rdfs:subClassOf rdf:nodeID="ub1bL187C19"/>
    <rdfs:subClassOf rdf:resource="http://www.w3.org/ns/sosa/Sample"/>
    <rdfs:comment>ownership is associated with the parent survey</rdfs:comment>
    <rdfs:subClassOf rdf:nodeID="ub1bL171C19"/>
    <rdfs:comment>rights and conditions are associated with the parnet survey</rdfs:comment>
    <rdfs:subClassOf rdf:resource="http://www.opengis.net/ont/geosparql#SpatialObject"/>
    <rdfs:subClassOf rdf:nodeID="ub1bL177C19"/>
    <rdfs:label>Site or location</rdfs:label>
    <rdfs:comment>Location where observations may be made&#13;
May be a plot, quadrat, transect, trap etc&#13;
&#13;
This is a sub-class of sosa:Sample because a site should be designed to to be representative of an environmental system (which may be an ecosystem or bioregion) or zone (which might be a fiat zone such as a parcel or tract)</rdfs:comment>
  </rdf:Description>
  <rdf:Description rdf:about="http://linked.data.gov.au/def/plot/SiteStratum">
    <rdfs:subClassOf rdf:nodeID="ub1bL218C19"/>
    <rdfs:subClassOf rdf:nodeID="ub1bL213C19"/>
    <rdfs:label>Vegetation stratum</rdfs:label>
    <rdf:type rdf:resource="http://www.w3.org/2002/07/owl#Class"/>
    <rdfs:comment>Structural element covering a recognisable height range in vegetation ecosystem occurring at an observation site</rdfs:comment>
    <rdfs:subClassOf rdf:resource="http://www.w3.org/ns/sosa/Sample"/>
    <rdfs:subClassOf rdf:nodeID="ub1bL208C19"/>
  </rdf:Description>
  <rdf:Description rdf:nodeID="ub1bL77C19">
    <owl:onProperty rdf:resource="http://linked.data.gov.au/def/plot/locationMethod"/>
    <owl:minCardinality rdf:datatype="http://www.w3.org/2001/XMLSchema#nonNegativeInteger">0</owl:minCardinality>
    <rdf:type rdf:resource="http://www.w3.org/2002/07/owl#Restriction"/>
  </rdf:Description>
  <rdf:Description rdf:nodeID="ub1bL87C19">
    <owl:onProperty rdf:resource="http://www.opengis.net/ont/geosparql#hasGeometry"/>
    <rdf:type rdf:resource="http://www.w3.org/2002/07/owl#Restriction"/>
    <owl:someValuesFrom rdf:resource="http://www.w3.org/2003/01/geo/wgs84_pos#Point"/>
  </rdf:Description>
  <rdf:Description rdf:nodeID="ub1bL411C19">
    <owl:onProperty rdf:resource="http://www.w3.org/ns/locn#location"/>
    <rdf:type rdf:resource="http://www.w3.org/2002/07/owl#Restriction"/>
    <owl:minCardinality rdf:datatype="http://www.w3.org/2001/XMLSchema#nonNegativeInteger">1</owl:minCardinality>
  </rdf:Description>
  <rdf:Description rdf:nodeID="ub1bL447C19">
    <rdf:type rdf:resource="http://www.w3.org/2002/07/owl#Restriction"/>
    <owl:minCardinality rdf:datatype="http://www.w3.org/2001/XMLSchema#nonNegativeInteger">1</owl:minCardinality>
    <owl:onProperty rdf:resource="http://purl.org/dc/elements/1.1/creator"/>
  </rdf:Description>
  <rdf:Description rdf:nodeID="ub1bL67C19">
    <owl:maxCardinality rdf:datatype="http://www.w3.org/2001/XMLSchema#nonNegativeInteger">1</owl:maxCardinality>
    <owl:onProperty rdf:resource="http://linked.data.gov.au/def/plot/mapsheetName"/>
    <rdf:type rdf:resource="http://www.w3.org/2002/07/owl#Restriction"/>
  </rdf:Description>
  <rdf:Description rdf:nodeID="f7656e68342664385b4e3faded1cecac5b5">
    <rdf:rest rdf:resource="http://www.w3.org/1999/02/22-rdf-syntax-ns#nil"/>
    <rdf:first rdf:resource="http://www.w3.org/ns/ssn/ext/ObservationCollection"/>
  </rdf:Description>
  <rdf:Description rdf:about="http://linked.data.gov.au/def/plot/mapsheetName">
    <rdfs:range rdf:resource="http://www.w3.org/2001/XMLSchema#string"/>
    <rdfs:label>Mapsheet</rdfs:label>
    <rdf:type rdf:resource="http://www.w3.org/2002/07/owl#DatatypeProperty"/>
  </rdf:Description>
  <rdf:Description rdf:about="http://www.w3.org/2003/01/geo/wgs84_pos#Point">
    <rdfs:subClassOf rdf:resource="http://www.opengis.net/ont/geosparql#Geometry"/>
    <rdfs:subClassOf rdf:resource="http://www.w3.org/ns/sosa/Result"/>
    <rdfs:subClassOf rdf:resource="http://www.w3.org/ns/locn#Geometry"/>
  </rdf:Description>
  <rdf:Description rdf:nodeID="ub1bL149C26">
    <owl:unionOf rdf:nodeID="f7656e68342664385b4e3faded1cecac5b1"/>
    <rdf:type rdf:resource="http://www.w3.org/2002/07/owl#Class"/>
  </rdf:Description>
  <rdf:Description rdf:about="http://linked.data.gov.au/def/plot/wasSubActivityOf">
    <rdfs:subPropertyOf rdf:resource="http://www.w3.org/ns/prov#wasInformedBy"/>
    <rdfs:label>pointer to parent activity</rdfs:label>
    <rdf:type rdf:resource="http://www.w3.org/2002/07/owl#ObjectProperty"/>
    <owl:inverseOf rdf:resource="http://linked.data.gov.au/def/plot/hadSubActivity"/>
  </rdf:Description>
  <rdf:Description rdf:nodeID="ub1bL157C19">
    <rdfs:comment>A site is established in the context of a site-visit, which is in turn part of a survey.&#13;
Different visits might create sites in the same place with different identifiers</rdfs:comment>
    <owl:allValuesFrom rdf:resource="http://linked.data.gov.au/def/plot/SiteVisit"/>
    <rdf:type rdf:resource="http://www.w3.org/2002/07/owl#Restriction"/>
    <owl:onProperty rdf:resource="http://www.w3.org/ns/sosa/isResultOf"/>
  </rdf:Description>
  <rdf:Description rdf:about="http://linked.data.gov.au/def/plot/mapScale">
    <rdf:type rdf:resource="http://www.w3.org/2002/07/owl#ObjectProperty"/>
    <rdfs:label>Map scale</rdfs:label>
  </rdf:Description>
  <rdf:Description rdf:about="http://linked.data.gov.au/def/plot/x/hasResultQuality">
    <rdfs:comment>this property allows an indication of the quality of the data to be provided at the level of either an individual observation or a thematic group. This is commonly done by some kind of description of the method, protocol, sensor, observer, etc. </rdfs:comment>
    <rdfs:domain rdf:nodeID="ub1bL494C15"/>
    <rdfs:label>Quality of individual or related observation results</rdfs:label>
    <rdf:type rdf:resource="http://www.w3.org/2002/07/owl#ObjectProperty"/>
  </rdf:Description>
  <rdf:Description rdf:about="http://linked.data.gov.au/def/plot/Stratum">
    <rdfs:label>Vegetation strata classification </rdfs:label>
    <rdf:type rdf:resource="http://www.w3.org/2002/07/owl#Class"/>
    <rdfs:comment>Structural element covering a recognisable height range in vegetation ecosystem</rdfs:comment>
    <rdfs:subClassOf rdf:resource="http://www.w3.org/2004/02/skos/core#Concept"/>
  </rdf:Description>
  <rdf:Description rdf:nodeID="f7656e68342664385b4e3faded1cecac5b9">
    <rdf:rest rdf:resource="http://www.w3.org/1999/02/22-rdf-syntax-ns#nil"/>
    <rdf:first rdf:resource="http://www.w3.org/2003/01/geo/wgs84_pos#Point"/>
  </rdf:Description>
  <rdf:Description rdf:about="http://linked.data.gov.au/def/plot/x/EcologicalCommunity">
    <rdfs:label>Ecological Community</rdfs:label>
    <rdf:type rdf:resource="http://www.w3.org/2002/07/owl#Class"/>
    <rdfs:subClassOf rdf:resource="http://linked.data.gov.au/def/plot/x/EnvironmentalSystem"/>
    <skos:closeMatch rdf:resource="http://purl.obolibrary.org/obo/PCO_0000002"/>
  </rdf:Description>
  <rdf:Description rdf:about="http://linked.data.gov.au/def/plot/x/sampleLevel">
    <rdfs:range rdf:resource="http://www.w3.org/2004/02/skos/core#Concept"/>
    <rdfs:label>sample level classification</rdfs:label>
    <rdfs:subPropertyOf rdf:resource="http://purl.org/dc/terms/type"/>
    <rdfs:domain rdf:resource="http://linked.data.gov.au/def/plot/Site"/>
    <rdf:type rdf:resource="http://www.w3.org/2002/07/owl#ObjectProperty"/>
  </rdf:Description>
  <rdf:Description rdf:about="http://www.w3.org/ns/ssn/ext/isMemberOf">
    <rdfs:range rdf:resource="http://www.w3.org/ns/ssn/ext/ObservationCollection"/>
    <rdfs:domain rdf:nodeID="ub1bL571C15"/>
    <owl:inverseOf rdf:resource="http://www.w3.org/ns/ssn/ext/hasMember"/>
    <rdfs:comment>indicates a collection of which the context resource is a member</rdfs:comment>
    <rdf:type rdf:resource="http://www.w3.org/2002/07/owl#ObjectProperty"/>
    <rdfs:label>is member of</rdfs:label>
    <rdfs:subPropertyOf rdf:resource="http://linked.data.gov.au/def/plot/wasSubActivityOf"/>
  </rdf:Description>
  <rdf:Description rdf:nodeID="ub1bL554C23">
    <owl:unionOf rdf:nodeID="f7656e68342664385b4e3faded1cecac5b8"/>
    <rdf:type rdf:resource="http://www.w3.org/2002/07/owl#Class"/>
  </rdf:Description>
  <rdf:Description rdf:about="http://linked.data.gov.au/def/plot/x/Assemblage">
    <rdfs:label>Organism assemblage</rdfs:label>
    <rdfs:subClassOf rdf:resource="http://linked.data.gov.au/def/plot/x/EcologicalCommunity"/>
    <rdf:type rdf:resource="http://www.w3.org/2002/07/owl#Class"/>
  </rdf:Description>
  <rdf:Description rdf:nodeID="ub1bL571C15">
    <owl:unionOf rdf:nodeID="f7656e68342664385b4e3faded1cecac5b10"/>
    <rdf:type rdf:resource="http://www.w3.org/2002/07/owl#Class"/>
  </rdf:Description>
  <rdf:Description rdf:nodeID="ub1bL458C19">
    <rdf:type rdf:resource="http://www.w3.org/2002/07/owl#Restriction"/>
    <owl:onProperty rdf:resource="http://purl.org/dc/terms/accessRights"/>
    <owl:onClass rdf:resource="http://www.w3.org/ns/odrl/2/Permission"/>
    <owl:qualifiedCardinality rdf:datatype="http://www.w3.org/2001/XMLSchema#nonNegativeInteger">1</owl:qualifiedCardinality>
  </rdf:Description>
  <rdf:Description rdf:nodeID="ub1bL218C19">
    <owl:onProperty rdf:resource="http://www.w3.org/ns/sosa/isFeatureOfInterestOf"/>
    <owl:minCardinality rdf:datatype="http://www.w3.org/2001/XMLSchema#nonNegativeInteger">1</owl:minCardinality>
    <rdf:type rdf:resource="http://www.w3.org/2002/07/owl#Restriction"/>
  </rdf:Description>
  <rdf:Description rdf:about="http://linked.data.gov.au/def/plot/x/EnvironmentalSystem">
    <rdfs:subClassOf rdf:resource="http://linked.data.gov.au/def/plot/x/EnvironmentalContinuant"/>
    <rdfs:label>Environmental region defined primarily by its function and membership</rdfs:label>
    <rdfs:subClassOf rdf:resource="http://www.w3.org/2002/07/owl#Thing"/>
    <rdf:type rdf:resource="http://www.w3.org/2002/07/owl#Class"/>
  </rdf:Description>
  <rdf:Description rdf:nodeID="ub1bL192C19">
    <rdf:type rdf:resource="http://www.w3.org/2002/07/owl#Restriction"/>
    <owl:minCardinality rdf:datatype="http://www.w3.org/2001/XMLSchema#nonNegativeInteger">1</owl:minCardinality>
    <owl:onProperty rdf:resource="http://linked.data.gov.au/def/plot/siteDescription"/>
  </rdf:Description>
  <rdf:Description rdf:about="http://linked.data.gov.au/def/plot/x/EnvironmentalContinuant">
    <rdfs:subClassOf rdf:resource="http://www.w3.org/ns/sosa/FeatureOfInterest"/>
    <rdf:type rdf:resource="http://www.w3.org/2002/07/owl#Class"/>
    <rdfs:label>Environmental continuant</rdfs:label>
    <skos:closeMatch rdf:resource="http://purl.obolibrary.org/obo/ENVO_01000408"/>
    <rdfs:comment>Union of environmental system, environmental zone, and ecological community?</rdfs:comment>
  </rdf:Description>
  <rdf:Description rdf:nodeID="ub1bL298C19">
    <rdf:type rdf:resource="http://www.w3.org/2002/07/owl#Restriction"/>
    <owl:allValuesFrom rdf:resource="http://linked.data.gov.au/def/plot/Site"/>
    <rdfs:comment>link to the visited site</rdfs:comment>
    <owl:onProperty rdf:resource="http://www.w3.org/ns/sosa/hasFeatureOfInterest"/>
  </rdf:Description>
  <rdf:Description rdf:nodeID="f7656e68342664385b4e3faded1cecac5b1">
    <rdf:rest rdf:nodeID="f7656e68342664385b4e3faded1cecac5b2"/>
    <rdf:first rdf:resource="http://linked.data.gov.au/def/plot/x/EnvironmentalSystem"/>
  </rdf:Description>
  <rdf:Description rdf:nodeID="ub1bL182C19">
    <owl:onProperty rdf:resource="http://www.w3.org/ns/prov#wasGeneratedBy"/>
    <rdf:type rdf:resource="http://www.w3.org/2002/07/owl#Restriction"/>
    <owl:allValuesFrom rdf:resource="http://www.w3.org/ns/prov#Activity"/>
  </rdf:Description>
  <rdf:Description rdf:nodeID="ub1bL442C19">
    <owl:onProperty rdf:resource="http://purl.org/dc/terms/title"/>
    <owl:cardinality rdf:datatype="http://www.w3.org/2001/XMLSchema#nonNegativeInteger">1</owl:cardinality>
    <rdf:type rdf:resource="http://www.w3.org/2002/07/owl#Restriction"/>
  </rdf:Description>
  <rdf:Description rdf:nodeID="ub1bL51C23">
    <rdf:type rdf:resource="http://www.w3.org/ns/prov#Activity"/>
    <doap:repository rdf:resource="https://bitbucket.org/terndatateam/ternplotdata-ontology"/>
    <rdf:type rdf:resource="http://usefulinc.com/ns/doap#Project"/>
  </rdf:Description>
  <rdf:Description rdf:nodeID="ub1bL478C19">
    <rdf:type rdf:resource="http://www.w3.org/2002/07/owl#Restriction"/>
    <owl:hasValue rdf:resource="http://www.tern.org.au/cv/op/Taxon-identity"/>
    <owl:onProperty rdf:resource="http://www.w3.org/ns/sosa/observedProperty"/>
  </rdf:Description>
  <rdf:Description rdf:nodeID="f7656e68342664385b4e3faded1cecac5b2">
    <rdf:rest rdf:resource="http://www.w3.org/1999/02/22-rdf-syntax-ns#nil"/>
    <rdf:first rdf:resource="http://linked.data.gov.au/def/plot/x/EnvironmentalZone"/>
  </rdf:Description>
  <rdf:Description rdf:nodeID="ub1bL464C19">
    <owl:onClass rdf:resource="http://www.w3.org/ns/odrl/2/Policy"/>
    <owl:qualifiedCardinality rdf:datatype="http://www.w3.org/2001/XMLSchema#nonNegativeInteger">1</owl:qualifiedCardinality>
    <rdf:type rdf:resource="http://www.w3.org/2002/07/owl#Restriction"/>
    <owl:onProperty rdf:resource="http://purl.org/dc/terms/license"/>
  </rdf:Description>
  <rdf:Description rdf:nodeID="ub1bL145C19">
    <rdf:type rdf:resource="http://www.w3.org/2002/07/owl#Restriction"/>
    <rdfs:comment>A Site is established to sample some biome, bioregion, ecosystem, etc.</rdfs:comment>
    <owl:onProperty rdf:resource="http://www.w3.org/ns/sosa/isSampleOf"/>
    <owl:someValuesFrom rdf:nodeID="ub1bL149C26"/>
  </rdf:Description>
  <rdf:Description rdf:nodeID="ub1bL124C19">
    <owl:onProperty rdf:resource="http://linked.data.gov.au/def/plot/taxon"/>
    <rdf:type rdf:resource="http://www.w3.org/2002/07/owl#Restriction"/>
    <owl:minCardinality rdf:datatype="http://www.w3.org/2001/XMLSchema#nonNegativeInteger">1</owl:minCardinality>
  </rdf:Description>
  <rdf:Description rdf:about="http://www.opengis.net/ont/geosparql#hasGeometry">
    <rdfs:subPropertyOf rdf:resource="http://www.w3.org/ns/locn#geometry"/>
  </rdf:Description>
  <rdf:Description rdf:nodeID="ub1bL494C15">
    <rdf:type rdf:resource="http://www.w3.org/2002/07/owl#Class"/>
    <owl:unionOf rdf:nodeID="f7656e68342664385b4e3faded1cecac5b6"/>
  </rdf:Description>
  <rdf:Description rdf:about="http://linked.data.gov.au/def/plot/x/TaxonAssignment">
    <rdf:type rdf:resource="http://www.w3.org/2000/01/rdf-schema#Class"/>
    <rdfs:label>Taxon assignment observation</rdfs:label>
    <rdfs:subClassOf rdf:resource="http://www.w3.org/ns/sosa/Observation"/>
    <rdfs:subClassOf rdf:nodeID="ub1bL478C19"/>
    <rdf:type rdf:resource="http://www.w3.org/2002/07/owl#Class"/>
  </rdf:Description>
  <rdf:Description rdf:nodeID="ub1bL82C19">
    <rdf:type rdf:resource="http://www.w3.org/2002/07/owl#Restriction"/>
    <owl:onProperty rdf:resource="http://www.opengis.net/ont/geosparql#hasGeometry"/>
    <owl:minCardinality rdf:datatype="http://www.w3.org/2001/XMLSchema#nonNegativeInteger">1</owl:minCardinality>
  </rdf:Description>
  <rdf:Description rdf:about="http://linked.data.gov.au/def/plot/SiteTaxon">
    <rdfs:subClassOf rdf:nodeID="ub1bL271C19"/>
    <rdfs:comment>Community of a single taxon in vegetation ecosystem occurring at an observation site</rdfs:comment>
    <rdf:type rdf:resource="http://www.w3.org/2002/07/owl#Class"/>
    <rdfs:comment>Data corresponding to an individual of this class would usually be derived from observations relating to the set of SiteStratumTaxon at the same site on the same taxon</rdfs:comment>
    <rdfs:subClassOf rdf:resource="http://www.w3.org/ns/sosa/Sample"/>
    <rdfs:label>Single taxon community</rdfs:label>
    <rdfs:subClassOf rdf:nodeID="ub1bL276C19"/>
    <rdfs:subClassOf rdf:nodeID="ub1bL281C19"/>
  </rdf:Description>
  <rdf:Description rdf:nodeID="ub1bL229C19">
    <owl:onProperty rdf:resource="http://linked.data.gov.au/def/plot/taxon"/>
    <owl:cardinality rdf:datatype="http://www.w3.org/2001/XMLSchema#nonNegativeInteger">1</owl:cardinality>
    <rdf:type rdf:resource="http://www.w3.org/2002/07/owl#Restriction"/>
    <rdfs:comment>While the value of the SiteStratumTaxon/taxon property might be fixed a-priori, the taxon-classification is typically the result of an observation whose feature-of-interest is an individual of the SiteStratumTaxon class. </rdfs:comment>
  </rdf:Description>
  <rdf:Description rdf:nodeID="ub1bL242C19">
    <owl:onProperty rdf:resource="http://www.w3.org/ns/sosa/isSampleOf"/>
    <rdfs:comment>relation to the SiteStratum for which this SiteStratumTaxon represents the community of a single taxon</rdfs:comment>
    <owl:someValuesFrom rdf:resource="http://linked.data.gov.au/def/plot/SiteStratum"/>
    <rdf:type rdf:resource="http://www.w3.org/2002/07/owl#Restriction"/>
  </rdf:Description>
  <rdf:Description rdf:about="http://linked.data.gov.au/def/plot/siteDescription">
    <rdfs:domain rdf:resource="http://linked.data.gov.au/def/plot/Site"/>
    <rdfs:range rdf:resource="http://www.w3.org/ns/ssn/ext/ObservationCollection"/>
    <rdf:type rdf:resource="http://www.w3.org/2002/07/owl#ObjectProperty"/>
    <rdfs:subPropertyOf rdf:resource="http://www.w3.org/ns/sosa/isFeatureOfInterestOf"/>
  </rdf:Description>
  <rdf:Description rdf:nodeID="ub1bL197C19">
    <owl:onProperty rdf:resource="http://purl.org/dc/terms/relation"/>
    <owl:someValuesFrom rdf:resource="http://linked.data.gov.au/def/plot/Site"/>
    <rdf:type rdf:resource="http://www.w3.org/2002/07/owl#Restriction"/>
  </rdf:Description>
  <rdf:Description rdf:nodeID="ub1bL171C19">
    <owl:allValuesFrom rdf:resource="http://linked.data.gov.au/def/plot/Site"/>
    <rdfs:comment>A site may be part of a bigger site -e.g. points within a plot</rdfs:comment>
    <owl:onProperty rdf:resource="http://purl.org/dc/terms/isPartOf"/>
    <rdf:type rdf:resource="http://www.w3.org/2002/07/owl#Restriction"/>
  </rdf:Description>
  <rdf:Description rdf:about="http://linked.data.gov.au/def/plot/hasLocation">
    <rdf:type rdf:resource="http://www.w3.org/2002/07/owl#ObjectProperty"/>
    <rdfs:label>has location</rdfs:label>
  </rdf:Description>
  <rdf:Description rdf:nodeID="ub1bL416C19">
    <owl:onClass rdf:resource="http://www.w3.org/ns/sosa/Sensor"/>
    <rdf:type rdf:resource="http://www.w3.org/2002/07/owl#Restriction"/>
    <owl:onProperty rdf:resource="http://www.w3.org/ns/sosa/hosts"/>
    <owl:minQualifiedCardinality rdf:datatype="http://www.w3.org/2001/XMLSchema#nonNegativeInteger">1</owl:minQualifiedCardinality>
  </rdf:Description>
  <rdf:Description rdf:nodeID="ub1bL292C19">
    <rdfs:comment>link from site-visit to survey of which it is a part</rdfs:comment>
    <rdf:type rdf:resource="http://www.w3.org/2002/07/owl#Restriction"/>
    <owl:onProperty rdf:resource="http://linked.data.gov.au/def/plot/wasSubActivityOf"/>
    <owl:someValuesFrom rdf:resource="http://linked.data.gov.au/def/plot/x/Survey"/>
  </rdf:Description>
  <rdf:Description rdf:about="http://linked.data.gov.au/def/plot/SiteVisit">
    <rdfs:label>Visit to a site</rdfs:label>
    <rdfs:subClassOf rdf:nodeID="ub1bL298C19"/>
    <rdfs:subClassOf rdf:nodeID="ub1bL292C19"/>
    <rdf:type rdf:resource="http://www.w3.org/2002/07/owl#Class"/>
    <rdfs:subClassOf rdf:nodeID="ub1bL304C19"/>
    <rdfs:subClassOf rdf:resource="http://www.w3.org/ns/prov#Activity"/>
    <rdfs:comment>A discrete time-bounded visit to a site, during which sampling or observation activities are undertaken</rdfs:comment>
  </rdf:Description>
  <rdf:Description rdf:nodeID="ub1bL165C19">
    <rdf:type rdf:resource="http://www.w3.org/2002/07/owl#Restriction"/>
    <owl:allValuesFrom rdf:resource="http://linked.data.gov.au/def/plot/Site"/>
    <rdfs:comment>A site may be part of a bigger site -e.g. points within a plot</rdfs:comment>
    <owl:onProperty rdf:resource="http://purl.org/dc/terms/hasPart"/>
  </rdf:Description>
  <rdf:Description rdf:nodeID="ub1bL177C19">
    <owl:allValuesFrom rdf:resource="http://linked.data.gov.au/def/plot/Location"/>
    <owl:onProperty rdf:resource="http://linked.data.gov.au/def/plot/hasLocation"/>
    <rdf:type rdf:resource="http://www.w3.org/2002/07/owl#Restriction"/>
  </rdf:Description>
  <rdf:Description rdf:nodeID="ub1bL119C19">
    <rdf:type rdf:resource="http://www.w3.org/2002/07/owl#Restriction"/>
    <owl:cardinality rdf:datatype="http://www.w3.org/2001/XMLSchema#nonNegativeInteger">1</owl:cardinality>
    <owl:onProperty rdf:resource="http://www.opengis.net/ont/geosparql#defaultGeometry"/>
  </rdf:Description>
  <rdf:Description rdf:about="http://linked.data.gov.au/def/plot/x/isLocationOf">
    <owl:inverseOf rdf:resource="http://www.w3.org/ns/locn#location"/>
    <rdfs:domain rdf:resource="http://linked.data.gov.au/def/plot/Location"/>
    <rdf:type rdf:resource="http://www.w3.org/2002/07/owl#ObjectProperty"/>
    <rdfs:comment>Links an individual location description to the resource (e.g. a plot:Site) that it relates to</rdfs:comment>
    <rdfs:label>describes the location of</rdfs:label>
  </rdf:Description>
  <rdf:Description rdf:nodeID="f7656e68342664385b4e3faded1cecac5b3">
    <rdf:rest rdf:nodeID="f7656e68342664385b4e3faded1cecac5b4"/>
    <rdf:first rdf:resource="http://www.w3.org/ns/sosa/Sampling"/>
  </rdf:Description>
  <rdf:Description rdf:nodeID="ub1bL430C19">
    <rdf:type rdf:resource="http://www.w3.org/2002/07/owl#Restriction"/>
    <owl:allValuesFrom rdf:resource="http://www.w3.org/2004/02/skos/core#Concept"/>
    <owl:onProperty rdf:resource="http://www.w3.org/ns/locn#location"/>
    <rdfs:comment>aka spatialScope? - to associate a jurisdiction or IBRA or other named thing with the Survey</rdfs:comment>
  </rdf:Description>
  <rdf:Description rdf:nodeID="ub1bL452C19">
    <owl:minQualifiedCardinality rdf:datatype="http://www.w3.org/2001/XMLSchema#nonNegativeInteger">1</owl:minQualifiedCardinality>
    <rdf:type rdf:resource="http://www.w3.org/2002/07/owl#Restriction"/>
    <owl:onProperty rdf:resource="http://www.w3.org/ns/sosa/hasFeatureOfInterest"/>
    <owl:onClass rdf:resource="http://linked.data.gov.au/def/plot/Site"/>
  </rdf:Description>
  <rdf:Description rdf:nodeID="ub1bL108C19">
    <owl:onProperty rdf:resource="http://www.w3.org/ns/sosa/isSampleOf"/>
    <rdfs:comment>An organism-occurrence is a sample of a community or assemblage</rdfs:comment>
    <rdf:type rdf:resource="http://www.w3.org/2002/07/owl#Restriction"/>
    <owl:someValuesFrom rdf:resource="http://linked.data.gov.au/def/plot/x/EcologicalCommunity"/>
  </rdf:Description>
  <rdf:Description rdf:about="http://www.w3.org/ns/locn#Geometry">
    <owl:equivalentClass rdf:nodeID="ub1bL554C23"/>
  </rdf:Description>
  <rdf:Description rdf:about="http://linked.data.gov.au/def/plot/mapsheetNumber">
    <rdfs:label>Mapsheet</rdfs:label>
    <rdf:type rdf:resource="http://www.w3.org/2002/07/owl#DatatypeProperty"/>
    <rdfs:range rdf:resource="http://www.w3.org/2001/XMLSchema#string"/>
  </rdf:Description>
  <rdf:Description rdf:about="http://linked.data.gov.au/def/plot/x/EnvironmentalZone">
    <rdfs:label>Environmental region defined primarily by its location and extent</rdfs:label>
    <rdfs:subClassOf rdf:resource="http://linked.data.gov.au/def/plot/x/EnvironmentalContinuant"/>
    <rdfs:subClassOf rdf:resource="http://www.w3.org/2002/07/owl#Thing"/>
    <rdf:type rdf:resource="http://www.w3.org/2002/07/owl#Class"/>
  </rdf:Description>
  <rdf:Description rdf:nodeID="ub1bL208C19">
    <rdf:type rdf:resource="http://www.w3.org/2002/07/owl#Restriction"/>
    <owl:allValuesFrom rdf:resource="http://linked.data.gov.au/def/plot/Site"/>
    <owl:onProperty rdf:resource="http://www.w3.org/ns/sosa/isSampleOf"/>
  </rdf:Description>
  <rdf:Description rdf:about="http://linked.data.gov.au/def/plot/x/floristics">
    <rdfs:subPropertyOf rdf:resource="http://purl.org/dc/terms/type"/>
    <rdfs:label>Site floristics classification</rdfs:label>
    <rdfs:domain rdf:resource="http://linked.data.gov.au/def/plot/Site"/>
    <rdfs:range rdf:resource="http://www.w3.org/2004/02/skos/core#Concept"/>
    <rdf:type rdf:resource="http://www.w3.org/2002/07/owl#ObjectProperty"/>
  </rdf:Description>
  <rdf:Description rdf:about="http://www.w3.org/ns/ssn/ext/hasMember">
    <rdfs:subPropertyOf rdf:resource="http://linked.data.gov.au/def/plot/hadSubActivity"/>
  </rdf:Description>
  <rdf:Description rdf:nodeID="ub1bL72C19">
    <owl:onProperty rdf:resource="http://linked.data.gov.au/def/plot/mapsheetNumber"/>
    <rdf:type rdf:resource="http://www.w3.org/2002/07/owl#Restriction"/>
    <owl:maxCardinality rdf:datatype="http://www.w3.org/2001/XMLSchema#nonNegativeInteger">1</owl:maxCardinality>
  </rdf:Description>
  <rdf:Description rdf:nodeID="ub1bL31C20">
    <sdo:name>CSIRO</sdo:name>
    <rdf:type rdf:resource="http://schema.org/Organization"/>
    <sdo:identifier rdf:resource="http://catalogue.linked.data.gov.au/def/csiro"/>
  </rdf:Description>
  <rdf:Description rdf:nodeID="ub1bL271C19">
    <rdf:type rdf:resource="http://www.w3.org/2002/07/owl#Restriction"/>
    <owl:onProperty rdf:resource="http://www.w3.org/ns/sosa/isSampleOf"/>
    <owl:allValuesFrom rdf:resource="http://linked.data.gov.au/def/plot/Site"/>
  </rdf:Description>
  <rdf:Description rdf:about="http://linked.data.gov.au/def/plot/locationMethod">
    <rdfs:label>Location method</rdfs:label>
    <rdf:type rdf:resource="http://www.w3.org/2002/07/owl#ObjectProperty"/>
  </rdf:Description>
  <rdf:Description rdf:nodeID="f7656e68342664385b4e3faded1cecac5b10">
    <rdf:rest rdf:nodeID="f7656e68342664385b4e3faded1cecac5b11"/>
    <rdf:first rdf:resource="http://www.w3.org/ns/sosa/Observation"/>
  </rdf:Description>
  <rdf:Description rdf:nodeID="f7656e68342664385b4e3faded1cecac5b6">
    <rdf:first rdf:resource="http://www.w3.org/ns/sosa/Observation"/>
    <rdf:rest rdf:nodeID="f7656e68342664385b4e3faded1cecac5b7"/>
  </rdf:Description>
  <rdf:Description rdf:about="http://linked.data.gov.au/def/plot/x/FluxTower">
    <rdfs:label>Flux tower</rdfs:label>
    <rdfs:subClassOf rdf:nodeID="ub1bL411C19"/>
    <rdf:type rdf:resource="http://www.w3.org/2002/07/owl#Class"/>
    <rdfs:subClassOf rdf:resource="http://www.w3.org/ns/sosa/Platform"/>
    <rdfs:subClassOf rdf:nodeID="ub1bL416C19"/>
    <rdf:type rdf:resource="http://www.w3.org/2000/01/rdf-schema#Class"/>
  </rdf:Description>
  <rdf:Description rdf:about="http://linked.data.gov.au/def/plot/x/observer">
    <rdfs:label>Observer</rdfs:label>
    <rdf:type rdf:resource="http://www.w3.org/2002/07/owl#ObjectProperty"/>
    <rdfs:subPropertyOf rdf:resource="http://www.w3.org/ns/prov#wasAssociatedWith"/>
    <rdfs:subPropertyOf rdf:resource="http://www.w3.org/ns/sosa/madeBySensor"/>
  </rdf:Description>
  <rdf:Description rdf:nodeID="f7656e68342664385b4e3faded1cecac5b7">
    <rdf:first rdf:resource="http://www.w3.org/ns/ssn/ext/ObservationCollection"/>
    <rdf:rest rdf:resource="http://www.w3.org/1999/02/22-rdf-syntax-ns#nil"/>
  </rdf:Description>
  <rdf:Description rdf:about="http://linked.data.gov.au/def/plot/x/visitor">
    <rdfs:label>Site visitor</rdfs:label>
    <rdf:type rdf:resource="http://www.w3.org/2002/07/owl#ObjectProperty"/>
    <rdfs:subPropertyOf rdf:resource="http://www.w3.org/ns/prov#wasAssociatedWith"/>
  </rdf:Description>
  <rdf:Description rdf:nodeID="ub1bL248C19">
    <rdf:type rdf:resource="http://www.w3.org/2002/07/owl#Restriction"/>
    <owl:onProperty rdf:resource="http://www.w3.org/ns/sosa/isSampleOf"/>
    <rdfs:comment>relation to the SiteTaxon for which this SiteStratumTaxon represents the community within a single stratum</rdfs:comment>
    <owl:someValuesFrom rdf:resource="http://linked.data.gov.au/def/plot/SiteTaxon"/>
  </rdf:Description>
  <rdf:Description rdf:about="https://bitbucket.org/terndatateam/ternplotdata-ontology">
    <rdf:type rdf:resource="http://usefulinc.com/ns/doap#Repository"/>
  </rdf:Description>
  <rdf:Description rdf:nodeID="ub1bL187C19">
    <rdf:type rdf:resource="http://www.w3.org/2002/07/owl#Restriction"/>
    <owl:cardinality rdf:datatype="http://www.w3.org/2001/XMLSchema#nonNegativeInteger">1</owl:cardinality>
    <owl:onProperty rdf:resource="http://purl.org/dc/terms/created"/>
  </rdf:Description>
</rdf:RDF>
